---
title: "Homework 2: problems about exponential families"
author: "TA : Arjama Das"
date: "Due: February 14th at 11:59 PM"
output: pdf_document
header-includes: 
 - \usepackage{amsthm}
 - \usepackage{amsmath}
 - \usepackage{amsfonts}
 - \usepackage{amscd}
 - \usepackage{amssymb}
 - \usepackage[sectionbib]{natbib}
 - \usepackage{url}
 - \usepackage{graphicx}
 - \usepackage{tikz-cd}
 - \usepackage{pgfplots}
 - \usepackage{geometry}
 - \usepackage{bm}
 - \usepackage{array,epsfig,fancyheadings,rotating}
 - \usepackage{multirow}
urlcolor: blue 
---

```{r setup, include=FALSE}
knitr::opts_chunk$set(echo = TRUE)
```

\newcommand{\R}{\mathbb{R}}

This homework set will cover problems concerning exponential family theory. All derivations must be typed. Screenshots of work done with pen and paper will not be accepted. 

\vspace*{1cm}

\noindent{\bf Problem 1} [10 points]: Verify that displayed equation 7 in the exponential family notes holds for the binomial distribution, the Poisson distribution, and the normal distribution with both $\mu$ and $\sigma^2$ unknown.

\vspace*{1cm}

\noindent{\bf Solution}:
(a) $Y \sim \operatorname{Bin}(n, p)$
$$
\begin{aligned}
\Longrightarrow f_{Y}(y) & =\binom{n}{y} p^{y}(1-p)^{n-y} \\
& =\binom{n}{y} e^{y \log p /(1-p)+n \log (1-p)}
\end{aligned}
$$

Thus,
$$
\begin{gathered}
\theta=\log \left(\frac{p}{1-p}\right) \\
c(\theta)=-n \log (1-p)=n \log \left(1+e^{\theta}\right)
\end{gathered}
$$

We know that,
$$
E_{\theta}(Y)=n p=n \frac{e^{\theta}}{1+e^{\theta}} ; \quad \operatorname{Var}_{\theta}(Y)=n p(1-p)=n \frac{e^{\theta}}{\left(1+e^{\theta}\right)^{2}}
$$

Now,
$$
\begin{aligned}
c^{\prime}(\theta) & =n \frac{1}{1+e^{\theta}} e^{\theta}=n p=E_{\theta}(Y) \\
c^{\prime \prime}(\theta) & =-n \frac{e^{2 \theta}}{\left(1+e^{\theta)^{2}}\right.}+n \frac{e^{\theta}}{1+e^{\theta}} \\
& =n \frac{e^{\theta}}{\left(1+e^{\theta}\right)^{2}} \\
& =n p(1-p) \\
& =\operatorname{Var}_{\theta}(Y)
\end{aligned}
$$

Thus equation (7) holds.

(b) $Y \sim \operatorname{Poi}(\lambda)$
$$
f_{Y}(y)=\frac{e^{-\lambda} \lambda^{y}}{y!}=e^{-\lambda+y \log \lambda -\log(x!)} 
$$

Thus,
$$
\theta=\log (\lambda) ; \quad c(\theta)=e^{\theta}
$$

We know that $E_{\theta}(Y)=\lambda=\operatorname{Var}_{\theta}(Y)$,
$$
c^{\prime}(\theta)=e^{\theta}=\lambda=E_{\theta}(Y) ; \quad c^{\prime \prime}(\theta)=e^{\theta}=\lambda=\operatorname{Var}_{\theta}(Y)
$$

Thus equation (7) holds.

(c) $Y \sim N\left(\mu, \sigma^{2}\right)$
$$
\begin{aligned}
f_{\mu, \sigma^{2}}(y) & =\frac{1}{\sqrt{2 \pi \sigma^{2}}} \exp \left(-\frac{(y-\mu)^{2}}{2 \sigma^{2}}\right) \\
& =\frac{1}{\sqrt{2 \pi \sigma^{2}}} \exp \left(-\frac{\left(y^{2}-2 y \mu+m u^{2}\right)}{2 \sigma^{2}}\right) \\
& =\frac{1}{\sqrt{2 \pi}} \exp \left(-\frac{y^{2}}{2 \sigma^{2}}+\frac{y \mu}{\sigma^{2}}-\frac{1}{2}\left(\frac{\mu^{2}}{\sigma^{2}}+\log \left(\sigma^{2}\right)\right)\right)
\end{aligned}
$$

Thus,
$$
Y(y)=\left(y,-y^{2}\right)^{T} ; \quad \theta=\left(\frac{\mu}{\sigma^{2}}, \frac{1}{2 \sigma^{2}}\right) ; \quad c(\theta)=\frac{1}{2}\left(\frac{\theta_{1}^{2}}{2 \theta_{2}}-\log \left(2 \theta_{2}\right)\right)
$$

We know that $\mathrm{E}(Y)=\mu, \mathrm{E}\left(Y^{2}\right)=\sigma^{2}+\mu^{2}, \operatorname{Var}(Y)=\sigma^{2}$ Let us now compute $\operatorname{Var}\left(Y^{2}\right)$.
The mgf of normal $N\left(\mu, \sigma^{2}\right)$ is $\exp \left(\mu t+\frac{\sigma^{2} t^{2}}{2}\right)$.
Thus,
$$
\begin{gathered}
M_{X}^{\prime}(t)=\exp \left(\mu t+\frac{\sigma^{2} t^{2}}{2}\right)\left(\mu+\sigma^{2} t\right) \\
\Longrightarrow M_{X}^{\prime \prime}(t)=\exp \left(\mu t+\frac{\sigma^{2} t^{2}}{2}\right)\left(\mu+\sigma^{2} t\right)^{2}+\exp \left(\mu t+\frac{\sigma^{2} t^{2}}{2}\right) \sigma^{2} \\
\Longrightarrow M_{X}^{(3)}(t)=\exp \left(\mu t+\frac{\sigma^{2} t^{2}}{2}\right)\left(\mu+\sigma^{2} t\right)^{3}+3 \exp \left(\mu t+\frac{\sigma^{2} t^{2}}{2}\right)\left(\mu+\sigma^{2} t\right) \sigma^{2} \\
\Longrightarrow M^{(4)}(t)=\exp \left(\mu t+\frac{\sigma^{2} t^{2}}{2}\right)\left(\mu+\sigma^{2} t\right)^{4}+6 \exp \left(\mu t+3 \frac{\sigma^{2} t^{2}}{2}\right)\left(\mu+\sigma^{2} t\right)^{2} \sigma^{2}+3 \exp \left(\mu t+\frac{\sigma^{2} t^{2}}{2}\right) \sigma^{4}
\end{gathered}
$$

Thus,
$$
\begin{gathered}
\mathrm{E}\left(Y^{3}\right)=\left.M_{X}^{(3)}(t)\right|_{t=0}=\mu^{3}+3 \mu \sigma^{2} \\
\mathrm{E}\left(Y^{4}\right)=\mu^{4}+6 \mu^{2} \sigma^{2}+3 \sigma^{4} \\
\Longrightarrow \operatorname{Var}\left(Y^{2}\right)=\mu^{4}+6 \mu^{2} \sigma^{2}+3 \sigma^{4}-\left(\sigma^{2}+\mu^{2}\right)^{2} \\
=\mu^{4}+6 \mu^{2} \sigma^{2}+3 \sigma^{4}-\sigma^{4}-\mu^{4}-2 \sigma^{2} \mu^{2}
\end{gathered}
$$
$$
=4 \mu^{2} \sigma^{2}+2 \sigma^{4}
$$
and,
$$
\operatorname{Cov}\left(Y, Y^{2}\right)=\mathrm{E}\left(Y^{3}\right)-\mathrm{E}\left(Y^{2}\right) \mathrm{E}(Y)=\mu^{3}+3 \mu \sigma^{2}-\mu\left(\sigma^{2}+\mu^{2}\right)=2 \mu \sigma^{2}
$$

Now,
$$
\begin{gathered}
c^{\prime}(\theta)=\left(\frac{\theta_{1}}{2 \theta_{2}},-\left(\frac{\theta_{1}^{2}}{4 \theta_{2}^{2}}+\frac{1}{2 \theta_{2}}\right)\right)=\left(\mu,-\mu^{2}-\sigma^{2}\right)=\left(\mathrm{E}(Y), \mathrm{E}\left(-Y^{2}\right)\right)=\mathrm{E}(Y(y)) \\
c^{\prime \prime}(\theta)=\left[\begin{array}{cc}
\frac{1}{2 \theta_{2}} & -\frac{\theta_{1}}{2 \theta_{2}^{2}} \\
-\frac{\theta_{1}}{2 \theta_{2}^{2}} & \frac{\theta_{1}^{2}}{2 \theta^{3}}+\frac{1}{2 \theta^{2}}
\end{array}\right]=\left[\begin{array}{cc}
\sigma^{2} & -2 \mu \sigma^{2} \\
-2 \mu \sigma^{2} & 4 \mu^{2} \sigma^{2}+2 \sigma^{4}
\end{array}\right]=\left[\begin{array}{cc}
\operatorname{Var}(Y) & \operatorname{Cov}\left(Y,-Y^{2}\right) \\
\operatorname{Cov}\left(Y,-Y^{2}\right) & \operatorname{Var}\left(Y^{2}\right)
\end{array}\right]=\operatorname{Var}(Y(y))
\end{gathered}
$$

Thus equation (7) holds.

\vspace*{1cm}

\noindent{\bf Problem 2} [20 points]: This problem concerns the proof of Theorem 3 in the exponential family notes. Do the following: 

- **part a** [10 points]: Show that the second derivative of the map $h$ is equal to $-\nabla^2 c(\theta)$ and justify that this matrix is negative definite when the exponential family model is identifiable.

\vspace*{1cm}

\noindent{\bf Solution}:
We know that,
$$
\begin{gathered}
h(\theta)=\langle\mu, \theta\rangle-c(\theta) \\
\Longrightarrow h^{\prime}(\theta)=\mu-\nabla c(\theta) \\
h^{\prime \prime}(\theta)=-\nabla^{2} c(\theta)=-\operatorname{Var}_{\theta}(Y)
\end{gathered}
$$

We know that $\operatorname{Var}_{\theta}(Y)$ is semi positive definite.
Consider a vector $x \neq 0$,
$$
\begin{aligned}
x^{T} \operatorname{Var}_{\theta}(Y) x & =x^{T}\left[\mathrm{E}_{\theta}\left(Y Y^{T}\right)-\mathrm{E}_{\theta}(Y) \mathrm{E}_{\theta}(Y)^{T}\right] x \\
& =\mathrm{E}_{\theta}\left(x^{T} Y Y^{T} x\right)-\mathrm{E}_{\theta}\left(x^{T} Y\right) \mathrm{E}_{\theta}\left(x^{T} Y\right)^{T} \\
& =\operatorname{Var}_{\theta}\left(x^{T} Y\right)
\end{aligned}
$$
$$
\therefore x^{T} \operatorname{Var}_{\theta}(Y) x=0 \Longrightarrow x^{T} Y=c \text { for any vector } x \neq 0 \text { and some const } \mathrm{c}
$$

But since the model is identifiable $x^{T} \operatorname{Var}_{\theta}(Y) x \neq 0$ for any non zero vector x . Thus $\operatorname{Var}_{\theta}(Y)$ is positive definite. Which implies that $-\nabla^{2} c(\theta)$ is negative definite.

\vspace*{1cm}

- **part b** [10 points]: Finish the proof of Theorem 3.

\vspace*{1cm}

\noindent{\bf Solution}:
The two steps that need to proof to complete the proof of the theorem are the following,

(a) The cumulant functions are infinitely differentiable and are therefore continuously differentiable.

Proof: We know that the moment generating function is infinitely differentiable. Since $\log$ is also an infinitely differentiable function and the cumulant generating function is the log of the moment generating function, the cumulant generating function is also infinitely differentiable. Consider $k_{\theta}(t)$ to be the cumulant generating function corresponding to the canonical statistic $\theta$ and $c(\theta)$ be the cumulant function, then we know that
$$
k_{\theta}(t)=c(t+\theta)-c(\theta)
$$

The derivatives of $k_{\theta}(t)$ evaluated at 0 are the same as the cumulant function c evaluated at $\theta$. Thus since the cumulant generating functions are infinitely differentiable, the cumulant functions are also infinitely differentiable and this further implies that the cumulant functions are also continuously differentiable.

(b) $g^{-1}(\theta)$ is infinitely differentiable

Proof: From the inverse function theorem we know that
$$
\nabla g^{-1}(\theta)=[\nabla g(\theta)]^{-1}
$$

Now note that $\nabla g(\theta)=\nabla^{2} c(\theta)$ and as shown above $\nabla^{2} c(\theta)$ is positive definite. Also $\frac{1}{x^{2}}$ is infinitely differentiable when $x \neq 0$. Thus $\left[\nabla^{2} c(\theta)\right]^{-1}$ is infinitely differentiable since $c(\theta)$ is infinitely differentiable (which would imply that $\nabla^{2} c(\theta)$ is also infinitely differentiable).
Combining the results: $\nabla g^{-1}(\theta)=[\nabla g(\theta)]^{-1}$ exists and is infinitely differentiable we get that $g^{-1}(\theta)$ is infinitely differentiable.


\vspace*{1cm}

Note that part a will be referenced later in this course. Hence, it is treated as its own sub-problem.

\vspace*{1cm}

\noindent{\bf Problem 3} [20 points]:  Let $y \in \R$ be a regular full exponential family with canonical parameter $\theta \in \R$. Do the following: 

- **part a** [15 points]: Verify that $y$ is sub-exponential.

\vspace*{1cm}

\noindent{\bf Solution}:
Need to show that Y is sub-exponential i.e. $\mathrm{E}\left(e^{\phi(Y-\mu)}\right) \leq e^{\lambda^{2} \phi^{2} / 2} \forall|\phi|<1 / b$ Using taylor expansion of $e^{x}$ we get,
$$
\begin{aligned}
\mathrm{E}(\exp \{\phi(Y-\mu)\}) & \approx E\left(1+\phi(Y-\mu)+\frac{\phi^{2}(Y-\mu)^{2}}{2}+O\left(\phi^{2}\right)\right) \\
& =1+\frac{\phi^{2} \operatorname{Var}_{\theta}(Y)}{2}+O\left(\phi^{2}\right)
\end{aligned}
$$

Similarly,
$$
e^{\lambda^{2} \phi^{2} / 2} \approx 1+\frac{\lambda^{2} \phi^{2}}{2}+O\left(\phi^{2}\right)
$$

Choosing a $\lambda$ such that $\operatorname{Var}_{\theta}(Y)<\lambda^{2}$ and b large enough such that $O\left(\phi^{2}\right)$ is negligible, for all $|\phi|<1 / b$ we get,
$$
\mathrm{E}(\exp \{\phi(Y-\mu)\}) \leq e^{\lambda^{2} \phi^{2} / 2}
$$

Thus, Y is sub-exponential.

\vspace*{1cm}

- **part b** [5 points]: In the notes it was claimed that the scalar products of $\sum_{i=1}^n\{y_i - \nabla c(\theta)\}$ are sub-exponential (see the "Finite sample concentration of MLE" section in the exponential family notes). Verify that this is true when $y_i$ are iid realizations from a regular full exponential family.

\vspace*{1cm}

\noindent{\bf Solution}:
Consider $\sum_{i=1}^{n} a_{i}\left\{y_{i}-\nabla c(\theta)\right\}$
Let $z_{i}=a_{i} y_{i}$. We know that $y_{i}$ is generated from an exponential family and thus $f_{Y_{i}}(y)=h(y) \exp \{\langle y, \theta\rangle-$ $c(\theta)\}$
Thus $f_{Z_{i}}(z)=\frac{h(z)}{a_{i}} \exp \left\{\left\langle z / a_{i}, \theta\right\rangle-c(\theta)\right\}$ which shows that $Z_{i}$ are also independent random variables from an exponential family with mean paramter $a_{i} \mu$
We have showed in the above problem that if Z is generated from a regular full exponential family then Z is sub-exponential.
$$
\Longrightarrow \mathrm{E}\left(\exp \left\{\phi_{i}\left(z_{i}-a_{i} \mu\right)\right\}\right) \leq \exp \left\{\frac{\lambda_{i}^{2} \phi_{i}^{2}}{2}\right\} \text { for some } \lambda_{i} \text { and } b_{i} \text { s.t it holds for all }\left|\phi_{i}\right|<1 / b_{i}
$$

Since $n$ is finite we can consider a b large enough such that $|\phi|<\frac{1}{b} \leq \frac{1}{b_{i}} \forall i$
$$
\begin{aligned}
\mathrm{E}\left(\exp \left\{\phi\left(\sum_{i=1}^{n} z_{i}-a_{i} \mu-0\right)\right\}\right) & =\prod_{i=1}^{n} \mathrm{E}\left(\exp \left\{\phi\left(z_{i}-a_{i} \mu\right)\right\}\right) \text { since independent } \\
& \leq \exp \left\{\frac{\phi^{2} \sum \lambda_{i}^{2}}{2}\right\} \\
& \text { Choosing a } \lambda \text { s.t. } \lambda^{2}=\sum_{i} \lambda_{i}^{2} \\
& =\exp \left\{\frac{\phi^{2} \lambda^{2}}{2}\right\}
\end{aligned}
$$

Thus, $\sum_{i=1}^{n} a_{i}\left\{y_{i}-\nabla c(\theta)\right\}$ is also sub-exponential.

\vspace*{1cm}

\noindent{\bf Problem 4} [10 points]: Derive the MLEs of the canonical parameters of the binomial distribution, and the normal distribution with both $\mu$ and $\sigma^2$ unknown.

\vspace*{1cm}

\noindent{\bf Solution}:
(a)A binomial random variable $Y \sim \text{Bin}(n, p)$ has the probability mass function:

$$
P(Y = y) = \binom{n}{y} p^y (1 - p)^{n - y}, \quad y = 0, 1, \dots, n.
$$



Given $m$ independent observations $y_1, y_2, \dots, y_m$ from $\text{Bin}(n, p)$, the likelihood function is:

$$
L(p) = \prod_{i=1}^{m} \binom{n}{y_i} p^{y_i} (1 - p)^{n - y_i}.
$$

Taking the log-likelihood:

$$
\ell(p) = \sum_{i=1}^{m} \log \binom{n}{y_i} + \sum_{i=1}^{m} y_i \log p + \sum_{i=1}^{m} (n - y_i) \log(1 - p).
$$

Ignoring constants:

$$
\ell(p) = \sum_{i=1}^{m} y_i \log p + \sum_{i=1}^{m} (n - y_i) \log(1 - p).
$$



Taking the derivative:

$$
\frac{d}{dp} \ell(p) = \sum_{i=1}^{m} \frac{y_i}{p} - \sum_{i=1}^{m} \frac{n - y_i}{1 - p}.
$$

Setting this to zero:

$$
\sum_{i=1}^{m} \frac{y_i}{p} = \sum_{i=1}^{m} \frac{n - y_i}{1 - p}.
$$

Solving for $p$:

$$
\hat{p} = \frac{\sum_{i=1}^{m} y_i}{m n} = \frac{\bar{y}}{n}.
$$



Rewriting in exponential family form:

$$
P(Y = y) = \exp\left( y \log \frac{p}{1 - p} + n \log(1 - p) + \log \binom{n}{y} \right).
$$

where the canonical parameter is:

$$
\theta = \log \frac{p}{1 - p}.
$$

Thus, the MLE for $\theta$ is:

$$
\hat{\theta} = \log \frac{\hat{p}}{1 - \hat{p}} = \log \frac{\bar{y}}{n - \bar{y}}.
$$

(b)A normal random variable $Y \sim \mathcal{N}(\mu, \sigma^2)$ has the probability density function:

$$
f(y) = \frac{1}{\sqrt{2\pi\sigma^2}} \exp\left(-\frac{(y - \mu)^2}{2\sigma^2} \right).
$$



Given $m$ independent observations $y_1, y_2, \dots, y_m$, the likelihood function is:

$$
L(\mu, \sigma^2) = \prod_{i=1}^{m} \frac{1}{\sqrt{2\pi\sigma^2}} \exp\left(-\frac{(y_i - \mu)^2}{2\sigma^2} \right).
$$

Taking the log-likelihood:

$$
\ell(\mu, \sigma^2) = -\frac{m}{2} \log(2\pi\sigma^2) - \frac{1}{2\sigma^2} \sum_{i=1}^{m} (y_i - \mu)^2.
$$


Differentiating with respect to $\mu$:

$$
\frac{d}{d\mu} \ell(\mu, \sigma^2) = \frac{1}{\sigma^2} \sum_{i=1}^{m} (y_i - \mu).
$$

Setting to zero:

$$
\sum_{i=1}^{m} (y_i - \hat{\mu}) = 0 \quad \Rightarrow \quad \hat{\mu} = \frac{1}{m} \sum_{i=1}^{m} y_i = \bar{y}.
$$



Differentiating with respect to $\sigma^2$:

$$
\frac{d}{d\sigma^2} \ell(\mu, \sigma^2) = -\frac{m}{2\sigma^2} + \frac{1}{2\sigma^4} \sum_{i=1}^{m} (y_i - \mu)^2.
$$

Setting to zero:

$$
\hat{\sigma}^2 = \frac{1}{m} \sum_{i=1}^{m} (y_i - \bar{y})^2.
$$



Rewriting the normal density function in exponential family form:

$$
f(y) = \exp\left( \frac{y\mu}{\sigma^2} - \frac{\mu^2}{2\sigma^2} - \frac{y^2}{2\sigma^2} - \frac{1}{2} \log (2\pi\sigma^2) \right).
$$

From this, the canonical parameters are:

$$
\theta_1 = \frac{\mu}{\sigma^2}, \quad \theta_2 = -\frac{1}{2\sigma^2}.
$$

Thus, the MLEs for the canonical parameters are:

$$
\hat{\theta}_1 = \frac{\hat{\mu}}{\hat{\sigma}^2} = \frac{\bar{y}}{\hat{\sigma}^2}, \quad \hat{\theta}_2 = -\frac{1}{2\hat{\sigma}^2} = -\frac{1}{2} \left( \frac{1}{m} \sum_{i=1}^{m} (y_i - \bar{y})^2 \right)^{-1}.
$$


\vspace*{1cm}

\noindent{\bf Problem 5} [10 points]: Derive the asymptotic distribution for $\hat\tau$, the MLE of the submodel mean value parameter vector. Hint: use the [Delta method](https://en.wikipedia.org/wiki/Delta_method).

\vspace*{1cm}

\noindent{\bf Solution}:
We know that the canonical linear submodel also has an exponential family with
- canonical statistic $M^{T} y$, cumulant function $\beta \rightarrow c(M \beta)$, and â€¢ submodel canonical parameter vector $\beta$.

And we know that for a exponential family with canonical statistic $Y^{*}$, canonical parameter $\theta$, mean parameter $\mu$ and cumulant function $c^{*}(\theta)$,
$$
\sqrt{n}\left(\bar{y}_{n}-\mu\right) \xrightarrow{d} N(0, I(\theta))
$$
and
$$
\sqrt{n}\left(\hat{\theta}_{n}-\theta\right) \xrightarrow{d} N\left(0, I(\theta)^{-1}\right)
$$

Using this we get,
$$
\sqrt{n}\left(M^{T}\left(\bar{y}_{n}\right)-\tau\right) \xrightarrow{d} N(0, I(\beta))
$$
where $I(\beta)=\nabla_{\beta}^{2} c(M \beta)=M^{T}\left[\left.\nabla_{\theta}^{2} c(\theta)\right|_{\theta=M \beta}\right] M$
and,
$$
\sqrt{n}(\hat{\beta}-\beta) \xrightarrow{d} N\left(0, I(\beta)^{-1}\right)
$$

\vspace*{1cm}

\noindent{\bf Problem 6} [20 points]: Do the following:  

- **part a** [10 points]: Prove Lemma 1 in the exponential family notes.

\vspace*{1cm}

\noindent{\bf Solution}:
The general form of an exponential family with canonical statistic X is
$$
f_{X}(x)=\underbrace{h(x)}_{f(x)} \underbrace{\exp \{\langle X, \theta\rangle-c(\theta)\}}_{g(X \mid \theta)}
$$

Thus, by the Neymann factorization Lemma, $X$ is the sufficient statistic.

\vspace*{1cm}

- **part b** [10 points]: Provide a brief explanation of why this Lemma is important without using any mathematical symbols.

\vspace*{1cm}

\noindent{\bf Solution}:
This lemma demonstrates a method for dimension reduction without any loss of information. In this case, we had a $n$-dimensional data reduced to a single value of $T = \sum Y_i$ while still preserving sufficient information according to Sufficiency Principle.

\vspace*{1cm} 
 
The above six problems are worth 90 points in total. 10 points will be allocated for presentation and correct submission of the homework.

\vspace*{1cm}



